Kraken/SeparationTests.lean
@@ -1,0 +1,33 @@
+import Kraken.SeparationTactics
+import Kraken.Mem
+
+open Std.ExtHashMap
+
+namespace Kraken.SeparationTests
+
+def indexed {w} (index : Nat) (p : Mem w → Prop) : Mem w → Prop :=
+  fun m => p m ∧ index = index
+
+example {w} (A B : Mem w → Prop) : A ⋆ B = B ⋆ A := by ecancel
+
+example {w} (A B : Mem w → Prop) : indexed 0 A ⋆ B = B ⋆ indexed 0 A := by ecancel
+
+example {w} (A B : Mem w → Prop) : emp ⋆ A ⋆ B = B ⋆ A := by ecancel
+
+example {w} (A B C D : Mem w → Prop) : A ⋆ (B ⋆ C) ⋆ D = (D ⋆ B) ⋆ (A ⋆ C) := by ecancel
+
+example {w} (A B C : Mem w → Prop) (m : Mem w) (h : (A ⋆ (B ⋆ C)) m) : ((C ⋆ A) ⋆ B) m := by ecancel
+
+example {w} (A : Mem w → Prop) : ∃ X : Mem w → Prop, A = X ⋆ A := by refine ⟨?_, by ecancel⟩
+
+example {w} (A B C : Mem w → Prop) : ∃ X : Mem w → Prop, A ⋆ (B ⋆ C) = X ⋆ A := by refine ⟨?_, by ecancel⟩
+
+example {w} (A B : Mem w → Prop) :
+    ∃ index : Nat, indexed index A ⋆ B = B ⋆ indexed 3 A := by
+  refine ⟨?_, by ecancel⟩
+
+example {w} (A : Mem w → Prop) :
+    ∃ x y : Nat, indexed x A ⋆ indexed 1 A = indexed y A ⋆ indexed 2 A := by
+  refine ⟨?_, ?_, by ecancel⟩
+
+end Kraken.SeparationTests
